TouhouFormal/ECL.lean
@@ -13,4 +13,5 @@ import TouhouFormal.ECL.Arithmetic
 import TouhouFormal.ECL.Assignment
 import TouhouFormal.ECL.Unary
 import TouhouFormal.ECL.FloatFunction
+import TouhouFormal.ECL.Random
 import TouhouFormal.ECL.Boss
