TouhouFormal/Search.lean
@@ -5,6 +5,7 @@ import TouhouFormal.Search.Difficulty
 import TouhouFormal.Search.FloatArithmetic
 import TouhouFormal.Search.FloatFunction
 import TouhouFormal.Search.IntUnaryUpdate
+import TouhouFormal.Search.Random
 import TouhouFormal.Search.ScalarAssignment
 import TouhouFormal.Search.SMT
 import TouhouFormal.Search.Symbolic
